---
title: "Exercise 2.8.16"
---

```{r include=FALSE} 
knitr::opts_chunk$set(options(scipen = 999))
knitr::opts_chunk$set(echo = FALSE)
```

> Use the definition of probability to verify rules:
> 
> (a) (2.4)

$\frac{n(S) - n(E)}{n(S)} = 1 - \frac{n(E)}{n(S)}$

> (b) (2.5)

$E$ and $F$ disjoint implies $n(E \cup F) = n(E) + n(F)$. So, probability of $E \cup F = \frac{n(E \cup F)}{n(S)} = \frac{n(E) + n(F)}{n(S)}$ and probability of $E$ $+$ probability of $F$ $=$ $\frac{n(E)}{n(S)} + \frac{n(F)}{n(S)}$.

> (c) (2.6)

$E$ and $F$ not disjoint implies $n(E \cup F) = n(E) + n(F) − n(E \cap F)$. So, probability of $E \cup F = \frac{n(E \cup F)}{n(S)} = \frac{n(E) + n(F) - n(E \cap F)}{n(S)}$ and probability of $E$ $+$ probability of $F$ $−$ probability of $E \cap F = \frac{n(E)}{n(S)} + \frac{n(F)}{n(S)} − \frac{n(E \cap F)}{n(S)}$.